Uppaal_Networks/UPPAAL_Asm_AbsInt_MapRefine.thy
@@ -12,10 +12,14 @@ fun r_lookup :: "('a::bot) r_state_map \<Rightarrow> addr \<Rightarrow> 'a" wher
 definition RSM :: "('a::bot) r_state_map \<Rightarrow> 'a state_map" where
   "RSM m = SM (r_lookup m)"
 
+declare RSM_def[simp]
+
 code_datatype RSM
 
-lemma[code]: "lookup (RSM m) = r_lookup m"
-  by (simp add: RSM_def)
+lemma[code]: "empty_map = RSM (Mapping.empty::('a::bot) r_state_map)"
+  by (rule lookup_eq; simp add: empty_map_def lookup_default_empty)
+
+lemma[code]: "lookup (RSM m) = r_lookup m" by simp
 
 fun merge_single :: "('a::sup) state_map \<Rightarrow> addr \<Rightarrow> 'a \<Rightarrow> 'a state_map" where
   "merge_single (SM m) pc x = SM (\<lambda>npc. if npc = pc then x \<squnion> m npc else m npc)"
@@ -23,20 +27,52 @@ fun merge_single :: "('a::sup) state_map \<Rightarrow> addr \<Rightarrow> 'a \<R
 fun r_merge_single :: "('a::{semilattice_sup, bot, linorder}) r_state_map \<Rightarrow> addr \<Rightarrow> 'a \<Rightarrow> 'a r_state_map" where
   "r_merge_single tree pc x = Mapping.update pc (x \<squnion> (r_lookup tree pc)) tree"
 
-lemma "pc \<noteq> ppc \<Longrightarrow> lookup (RSM (r_merge_single m pc x)) k = lookup (RSM m) k" sorry
+lemma merge_single_neq:
+  assumes "pc \<noteq> k"
+  shows "lookup (RSM (r_merge_single m pc x)) k = lookup (RSM m) k"
+proof -
+  have r: "lookup (RSM m) k = Mapping.lookup_default \<bottom> m k" by (simp add: RSM_def)
+  from assms have l:"lookup (RSM (r_merge_single m pc x)) k = Mapping.lookup_default \<bottom> m k" by (simp add: lookup_default_update_neq) 
+  from r l show ?thesis by simp
+qed
+
+lemma merge_single_eq:
+  assumes "pc = k"
+  shows "lookup (RSM (r_merge_single m pc x)) k = x \<squnion> lookup (RSM m) k"
+proof -
+  have r: "x \<squnion> lookup (RSM m) k = x \<squnion> Mapping.lookup_default \<bottom> m k" by simp
+  from assms have l:"lookup (RSM (r_merge_single m pc x)) k = x \<squnion> Mapping.lookup_default \<bottom> m k" by (simp add: lookup_default_update) 
+  from r l show ?thesis by simp
+qed
 
 lemma[code]: "merge_single (RSM m) pc x = RSM (r_merge_single m pc x)"
 proof(rule lookup_eq)
   obtain mm where func: "RSM m = SM mm" using state_map_single_constructor by blast
   have "(if k = pc then x \<squnion> mm k else mm k) = lookup (RSM (r_merge_single m pc x)) k" for k
   proof(cases "k = pc")
-    case True
-    then show ?thesis sorry
-  next
-    case False
-    then show ?thesis sorry
+    case True from this func show ?thesis using merge_single_eq by (metis lookup.simps) next
+    case False from this func show ?thesis using merge_single_neq by (metis lookup.simps)
   qed
-  thus "lookup (merge_single (RSM m) pc x) k = lookup (RSM (r_merge_single m pc x)) k" for k by (simp add: func)
+  thus "lookup (merge_single (RSM m) pc x) k = lookup (RSM (r_merge_single m pc x)) k" for k using func by auto
 qed
+
+fun r_domain :: "('b::bot) r_state_map \<Rightarrow> addr set" where
+  "r_domain tree = Set.filter (\<lambda>pc. r_lookup tree pc \<noteq> \<bottom>) (Mapping.keys tree)"
+
+lemma[code]: "domain (RSM m) = r_domain m"
+proof (intro Set.equalityI Set.subsetI)
+  fix x assume "x \<in> domain (RSM m)"
+  hence lookup: "lookup (RSM m) x \<noteq> \<bottom>" by simp
+  from lookup have r_lookup: "r_lookup m x \<noteq> \<bottom>" by simp
+  hence keys: "x \<in> Mapping.keys m"
+    by (metis Option.is_none_def empty_iff keys_empty keys_is_none_rep lookup_default_def lookup_default_empty r_lookup.simps)
+  from keys r_lookup show "x \<in> r_domain m" by auto
+qed auto
+
+value "
+  let m = empty_map::bool state_map;
+      m2 = merge_single m 42 True;
+      m3 = merge_single m2 123 False in
+  domain m3"
 
 end
